src/PlutusIR/Analysis/Purity.v
@@ -62,7 +62,7 @@ Definition is_pureb (Γ : ctx) (t : Term) : bool :=
       | Datatypes.Some (let_bound NonStrict) => false
       | _ => false
     end
-  | _     => is_value t && negb (is_errorb t)
+  | _     => dec_value t && negb (is_errorb t)
   end
 .
 
@@ -86,7 +86,7 @@ Inductive pure_binding (Γ : ctx) : Binding -> Prop :=
 Definition is_pure_binding (Γ : ctx) (b : Binding) : bool :=
     match b with
       | TermBind NonStrict vd t => true
-      | TermBind Strict vd t    => is_value t
+      | TermBind Strict vd t    => dec_value t
       | DatatypeBind dtd        => true
       | TypeBind tvd ty         => true
     end
